src/lang/Progress.v
@@ -19,21 +19,20 @@ Set Implicit Arguments.
 
 
 Lemma write_step_promise
-      lc1 sc1 mem1 loc from to val releasedm released ord lc2 sc2 mem2 kind
-      (STEP: Local.write_step lc1 sc1 mem1 loc from to val releasedm released ord lc2 sc2 mem2 kind)
+      lc1 sc1 mem1 loc from to val releasedm ord lc2 sc2 mem2
+      (STEP: Local.write_step lc1 sc1 mem1 loc from to val releasedm ord lc2 sc2 mem2)
       (PROMISES: lc1.(Local.promises) = Memory.bot):
   lc2.(Local.promises) = Memory.bot.
 Proof.
-  inv STEP.
-  - inv FULFILL. rewrite PROMISES in *. inv FULFILL0.
-    exploit Memory.remove_disjoint; eauto. rewrite Memory.bot_get. congr.
-  - apply Memory.ext. i. rewrite Memory.bot_get.
-    destruct (Memory.get loc0 ts (Local.promises lc2)) as [[]|] eqn:X; auto.
-    inv FULFILL. ss. inv FULFILL0. eapply Memory.remove_get_inv in X; eauto. des.
-    inv PROMISE. ss. eapply Memory.promise_promises_get2 in X0; eauto. des.
-    + subst. contradict X. auto.
-    + rewrite PROMISES, Memory.bot_get in *. congr.
-Qed.
+  inv STEP. rewrite PROMISES in *. s.
+  apply Memory.ext. i. rewrite Memory.bot_get.
+  destruct (Memory.get loc0 ts promises2) as [[]|] eqn:X; auto.
+  inv WRITE.
+  exploit Memory.remove_get_inv; eauto. i. des.
+  exploit Memory.promise_promises_get2; eauto. i. des.
+  - subst. contradict x0. auto.
+  - rewrite Memory.bot_get in *. congr.
+Admitted.
 
 Lemma program_step_promise
       lang e
@@ -43,7 +42,7 @@ Lemma program_step_promise
       (PROMISES: lc1.(Local.promises) = Memory.bot):
   lc2.(Local.promises) = Memory.bot.
 Proof.
-  inv STEP; try by inv LOCAL.
+  inv STEP; (try by inv LOCAL); eauto.
   - eapply write_step_promise; eauto.
   - eapply write_step_promise; eauto.
     inv LOCAL1. auto.
@@ -104,17 +103,6 @@ Proof.
           (try by unfold TimeMap.singleton, LocFun.add; condtac; [refl|congr]);
           (try by left; eapply TimeFacts.le_lt_lt; [|eauto];
            eapply closed_timemap_max_ts; apply WF1).
-  - refl.
-  - apply WF1.
-  - eapply Commit.future_closed; try apply WF1; eauto.
-Qed.
-
-Lemma progress_silent_step
-      lc1 mem1
-      (WF1: Local.wf lc1 mem1):
-  Local.silent_step lc1 mem1 lc1.
-Proof.
-  destruct lc1. econs; try apply WF1. refl.
 Qed.
 
 Lemma progress_read_step
@@ -131,23 +119,6 @@ Proof.
   eexists _, _, _. econs; eauto.
 Qed.
 
-Lemma progress_fulfill_step
-      lc1 sc1 mem1
-      loc from to val releasedm released ord
-      (LT: Time.lt from to)
-      (PROMISES1: lc1.(Local.promises) = Memory.singleton loc val released LT)
-      (RELEASED: Capability.join
-                   releasedm
-                   (Commit.rel
-                      (Commit.write_commit (Local.commit lc1) sc1 loc to ord) loc) =
-                 released):
-  exists lc2 sc2,
-    Local.fulfill_step lc1 sc1 mem1 loc from to val releasedm released ord lc2 sc2.
-Proof.
-  eexists _, _. econs; eauto.
-  rewrite PROMISES1. econs. apply Memory.remove_singleton.
-Qed.
-
 Lemma progress_write_step
       lc1 sc1 mem1
       loc to val releasedm ord
@@ -159,18 +130,16 @@ Lemma progress_write_step
       (CLOSED_REL: Memory.closed_capability releasedm mem1)
       (PROMISES1: lc1.(Local.promises) = Memory.bot):
   exists lc2 sc2 mem2,
-    Local.write_step lc1 sc1 mem1 loc (Memory.max_ts loc mem1) to val releasedm
-                     (Capability.join releasedm (Commit.rel (Commit.write_commit (Local.commit lc1) sc1 loc to ord) loc))
-                     ord lc2 sc2 mem2 Local.write_kind_promise_fulfill.
+    Local.write_step lc1 sc1 mem1 loc (Memory.max_ts loc mem1) to val releasedm ord lc2 sc2 mem2.
 Proof.
   exploit progress_promise_step; eauto. i. des.
-  exploit Local.promise_step_future; eauto. i. des.
+  exploit Local.promise_step_future; eauto. i. des. inv x0.
   assert (PROMISES2:
             promises2 = Memory.singleton
                           loc val
                           (Capability.join releasedm (Commit.rel (Commit.write_commit (Local.commit lc1) sc1 loc to ord) loc))
                           LT).
-  { inv x0. apply Memory.ext. i.
+  { apply Memory.ext. i.
     rewrite Memory.singleton_get. repeat condtac; subst.
     - destruct (Memory.get loc to promises2) as [[]|] eqn:X.
       + exploit Memory.promise_promises_get2; eauto. i. des; subst; eauto.
@@ -185,10 +154,9 @@ Proof.
       + congr.
       + rewrite PROMISES1, Memory.bot_get in *. congr.
   }
-  hexploit progress_fulfill_step; eauto.
-  { instantiate (7 := Local.mk _ _). apply PROMISES2. }
-  i. des. eexists _, _, _. econs; eauto.
-  rewrite PROMISES1. auto.
+  esplits. econs; eauto.
+  - econs; eauto. subst promises2. apply Memory.remove_singleton.
+  - rewrite PROMISES1. auto.
 Qed.
 
 Lemma progress_fence_step
